Leansubst/Defs.lean
@@ -27,206 +27,52 @@ inductive Expr (σ : Type) where
   | node   : σ → List (Expr σ) → Expr σ -- Tree node.
 
 /-- Substitutions. -/
-inductive Subst' (σ : Type) where
-  | shift : Nat →               Subst' σ -- Shift overflow variables up.
-  | cons  : Expr σ → Subst' σ → Subst' σ -- Prepend to sequence.
-
-namespace Subst'
-
-/-- The identity substitution. -/
-def id (σ) : Subst' σ :=
-  shift 0
-
-/-- Extract first element in sequence. -/
-def head : Subst' σ → Expr σ
-  | shift n  => .var n
-  | cons h _ => h
-
-/-- Drops first element in sequence. -/
-def tail : Subst' σ → Subst' σ
-  | shift n  => shift (n + 1)
-  | cons _ t => t
-
-/-- Drops first `n` elements in sequence. -/
-def drop : Nat → Subst' σ → Subst' σ
-  | 0,     s => s
-  | n + 1, s => tail (drop n s)
-
-/-- Get element at given index. -/
-def get : Nat → Subst' σ → Expr σ :=
-  fun n s => head (drop n s)
-
-/-- Extensional equivalence of substitutions. -/
-instance setoid (σ) : Setoid (Subst' σ) where
-  r     := fun s t => ∀ i, s.get i = t.get i
-  iseqv :=
-  { refl  := fun _ _ => .refl _
-    symm  := fun h i => .symm (h i)
-    trans := fun h₁ h₂ i => .trans (h₁ i) (h₂ i) }
-
-/-!
-  Instructions for the `simp` tactic.
--/
-
-@[simp↓ high] theorem id_expand : id σ = shift 0 := rfl
-@[simp low] theorem shift_zero : shift 0 = id σ := rfl
-@[simp high] theorem head_shift (n) : @head σ (shift n) = .var n := rfl
-@[simp high] theorem head_cons (h t) : @head σ (cons h t) = h := rfl
-@[simp↓ high] theorem tail_expand (s) : @tail σ s = drop 1 s := rfl
-@[simp low] theorem drop_one (s) : @drop σ 1 s = tail s := rfl
-
-@[simp high] theorem drop_zero (s) : @drop σ 0 s = s := rfl
-@[simp high] theorem drop_drop (n m s) : @drop σ n (drop m s) = drop (m + n) s := by
-  induction n with | zero => rfl | succ _ ih => rw [drop, ih, tail]; rfl
-@[simp high] theorem drop_shift (n m) : @drop σ n (shift m) = shift (m + n) := by
-  induction n with | zero => rfl | succ _ ih => rw [drop, ih, tail]; rfl
-@[simp high] theorem drop_cons (n h t) : @drop σ (n + 1) (cons h t) = drop n t := by
-  induction n with | zero => rfl | succ _ ih => rw [drop, ih, tail]; rfl
-
-@[simp↓ high] theorem get_expand (n s) : @get σ n s = head (drop n s) := rfl
-@[simp low] theorem head_drop (s n) : @head σ (drop n s) = get n s := rfl
-
-/-- Shift variables with level ≥ `n` by `m` levels (ugly bootstrapping definition). -/
-def applys : Nat → Nat → Expr σ → Expr σ
-  | n, m, .var i     => if n <= i then .var (i + m) else .var i
-  | n, m, .binder e  => .binder (applys (n + 1) m e)
-  | n, m, .node x es => .node x (nested n m es)
-where nested : Nat → Nat → List (Expr σ) → List (Expr σ)
-  | _, _, []      => []
-  | n, m, e :: es => applys n m e :: nested n m es
-
-/-- Composition of substitution and shift (ugly bootstrapping definition). -/
-def comps : Subst' σ → Nat → Subst' σ
-  | shift n,  m => .shift (n + m)
-  | cons h t, m => cons (applys 0 m h) (comps t m)
-
-/-- Composition of substitution and shift follows the expected definition. -/
-theorem comps_def (s : Subst' σ) (n : Nat) : ∀ i, get i (comps s n) = applys 0 n (get i s) := by
-  intros i
-  induction s generalizing i with
-  | shift m =>  
-    simp only [get, head, comps, drop_shift, applys, Nat.zero_le, ite_true]
-    rw [Nat.add_assoc, Nat.add_comm n i, ← Nat.add_assoc] 
-  | cons h s ih =>
-    simp only [comps, get_expand] at *
-    cases i with
-    | zero => rfl
-    | succ i => simp only [drop_cons] at *; rw [ih]
-
-/-- Applies a substitution on a term. -/
-def apply : Subst' σ → Expr σ → Expr σ
-  | s, .var i     => get i s
-  | s, .binder e  => .binder (apply (cons (.var 0) (comps s 1)) e)
-  | s, .node n es => .node n (nested s es)
-where nested : Subst' σ → List (Expr σ) → List (Expr σ)
-  | _, []      => []
-  | s, e :: es => apply s e :: nested s es
-termination_by
-  apply s e   => (sizeOf e, sizeOf s)
-  nested s es => (sizeOf es, sizeOf s)
-
-/-- Composition of substitutions. -/
-def comp : Subst' σ → Subst' σ → Subst' σ
-  | shift n,  r => drop n r
-  | cons h t, r => cons (apply r h) (comp t r)
-
-/-- Composition of substitutions follows the expected definition. -/
-theorem comp_def (s t : Subst' σ) : ∀ i, get i (comp s t) = apply t (get i s) := by
-  intros i
-  induction s generalizing t i with
-  | shift n => simp only [comp, get_expand, drop_drop, drop_shift, head_shift, apply]
-  | cons h s ih =>
-    simp only [comp, get_expand] at *
-    cases i with
-    | zero => rfl
-    | succ i => simp only [drop_cons]; rw [ih]
-
-/-- Now we can write `s t` for applying substitution `s` on term `t`. -/
-instance : CoeFun (Subst' σ) (fun _ => Expr σ → Expr σ) where
-  coe := apply
-
-end Subst'
-
-/-- Substitution modulo extensional equivalence. -/
 def Subst (σ : Type) : Type :=
-  Quotient (Subst'.setoid σ)
+  Nat → Expr σ
 
 namespace Subst
 
-local notation:arg "⟦" a "⟧" => Quotient.mk (Subst'.setoid _) a
-
-/-- Lifted constructor `shift`. -/
-def shift (σ) : Nat → Subst σ :=
-  fun n => ⟦Subst'.shift n⟧
-
-/-- Lifted constructor `cons`. -/
-def cons : Expr σ → Subst σ → Subst σ :=
-  fun e => Quotient.lift (fun s => ⟦Subst'.cons e s⟧) $ by
-    intros s t h
-    apply Quotient.sound; intros i
-    cases i with
-    | zero => rfl
-    | succ i => simp only [Subst'.get_expand, Subst'.drop_cons]; exact h i
-
-/-- Lifted constructor `id`. -/
+/-- The identity substitution. -/
 def id (σ) : Subst σ :=
-  ⟦Subst'.id σ⟧
+  fun i => .var i
 
-/-- Evaluate substitution at a given index. -/
-def get : Nat → Subst σ → Expr σ :=
-  fun n => Quotient.lift (Subst'.get n) $
-    fun _ _ h => h n
+/-- Shift overflow variables up. -/
+def shift (σ) : Nat → Subst σ :=
+  fun n i => .var (n + i)
 
-/-- Composition of substitution and shift. -/
-def comps : Subst σ → Nat → Subst σ :=
-  Quotient.lift (fun s n => ⟦Subst'.comps s n⟧) respects
-where
-  respects (s t : Subst' σ) (h : s ≈ t) : _ := by
-    apply funext; intros n
-    apply Quotient.sound; intros i
-    rw [Subst'.comps_def, Subst'.comps_def, h i]
+/-- Prepend to sequence. -/
+def cons : Expr σ → Subst σ → Subst σ :=
+  fun e f => fun | 0 => e | i + 1 => f i
+
+/-- Applies a renaming on a term. -/
+def applyr : (Nat → Nat) → Expr σ → Expr σ
+  | r, .var i     => .var (r i)
+  | r, .binder e  => .binder (applyr (fun | 0 => 0 | i + 1 => r i + 1) e)
+  | r, .node x es => .node x (nested r es)
+where nested : (Nat → Nat) → List (Expr σ) → List (Expr σ)
+  | _, []      => []
+  | r, e :: es => applyr r e :: nested r es
+
+/-- Composition of substitution and renaming. -/
+def compr : Subst σ → (Nat → Nat) → Subst σ :=
+  fun s r i => applyr r (s i)
 
 /-- Applies a substitution on a term. -/
-def apply : Subst σ → Expr σ → Expr σ :=
-  Quotient.lift Subst'.apply respects
-where
-  respects (s t : Subst' σ) (h : s ≈ t) : _ := by
-    apply funext; intros e; revert s t
-    -- Induction on `e`.
-    let motive := fun (e : Expr σ) => ∀ (s t : Subst' σ), s ≈ t → s e = t e
-    apply @Expr.recOn _ (fun e => motive e) (List.foldr (fun e etc => motive e ∧ etc) True)
-      <;> intros <;> (try trivial) <;> intros s t h
-    case var i => simp only [Subst'.apply, h i]
-    case binder e' ih =>
-      simp only [Subst'.apply]; congr 1
-      apply ih
-      apply Quotient.exact
-      suffices h : cons (.var 0) (comps ⟦s⟧ 1) = cons (.var 0) (comps ⟦t⟧ 1) by exact h
-      suffices h : ⟦s⟧ = ⟦t⟧ by rw [h]
-      exact Quotient.sound h
-    case node n es ih =>
-      induction es with
-      | nil => simp only [Subst'.apply, Subst'.apply.nested]
-      | cons h' t' ih' =>
-        rw [List.foldr] at ih
-        simp only [Subst'.apply, Subst'.apply.nested]
-        congr 2
-        . exact ih.left _ _ h
-        . specialize ih' ih.right
-          simp only [Subst'.apply] at ih'
-          injection ih'
+def apply : Subst σ → Expr σ → Expr σ
+  | s, .var i     => s i
+  | s, .binder e  => .binder (apply (cons (.var 0) (compr s (. + 1))) e)
+  | s, .node n es => .node n (nested s es)
+where nested : Subst σ → List (Expr σ) → List (Expr σ)
+  | _, []      => []
+  | s, e :: es => apply s e :: nested s es
 
 /-- Composition of substitutions. -/
 def comp : Subst σ → Subst σ → Subst σ :=
-  Quotient.lift₂ (fun s t => ⟦Subst'.comp s t⟧) respects
-where
-  respects (s₁ t₁ s₂ t₂ : Subst' σ) (h₁ : s₁ ≈ s₂) (h₂ : t₁ ≈ t₂) : _ := by
-    apply Quotient.sound; intros i
-    rw [Subst'.comp_def, Subst'.comp_def, h₁ i, apply.respects]; exact h₂
+  fun s t i => apply t (s i)
 
-/-- Now we can write `s t` for applying substitution `s` on term `t`. -/
-instance : CoeFun (Subst σ) (fun _ => Expr σ → Expr σ) where
-  coe := apply
+/-- Composition of substitutions follows the expected definition. -/
+@[simp]
+theorem comp_def (s t : Subst σ) : comp s t = apply t ∘ s := rfl
 
 end Subst
 
@@ -263,12 +109,12 @@ def SE.id (σ) : SE σ :=
 /-- Metavariable assignment. -/
 structure Assignment (σ : Type) where
   es : Nat → Expr σ
-  se : Nat → Subst' σ
+  se : Nat → Subst σ
 
 mutual
 /-- Assign metavariables. -/
 def ES.assign : Assignment σ → ES σ → Expr σ
-  | a, .subst e s => Subst'.apply (SE.assign a s) (ES.assign a e)
+  | a, .subst e s => Subst.apply (SE.assign a s) (ES.assign a e)
   | _, .zero      => .var 0
   | a, .binder e  => .binder (ES.assign a e)
   | a, .node n es => .node n (nested a es)
@@ -278,10 +124,10 @@ where nested : Assignment σ → List (ES σ) → List (Expr σ)
   | a, e :: es    => ES.assign a e :: nested a es
 
 /-- Assign metavariables. -/
-def SE.assign : Assignment σ → SE σ → Subst' σ
-  | _, .shift     => .shift 1
-  | a, .cons h t  => .cons (ES.assign a h) (SE.assign a t)
-  | a, .comp s t  => .comp (SE.assign a s) (SE.assign a t)
+def SE.assign : Assignment σ → SE σ → Subst σ
+  | _, .shift     => Subst.shift _ 1
+  | a, .cons h t  => Subst.cons (ES.assign a h) (SE.assign a t)
+  | a, .comp s t  => Subst.comp (SE.assign a s) (SE.assign a t)
   | a, .mvar i    => a.se i
 end
 
